scaffolding to make runnable kernels

compiler/dsl/ml/primitives/Main.ml
@@ -1,0 +1,1 @@
+STImpl.exec (Reflex.main []) ()
