compiler/dsl/ml/primitives/STImpl.ml
@@ -1,0 +1,55 @@
+(* Copyright (c) 2009, Harvard University
+ * All rights reserved.
+ *
+ * Authors: Gregory Malecha, Ryan Wisnesky
+ *
+ * Redistribution and use in source and binary forms, with or without
+ * modification, are permitted provided that the following conditions are met:
+ *
+ * - Redistributions of source code must retain the above copyright notice,
+ *   this list of conditions and the following disclaimer.
+ * - Redistributions in binary form must reproduce the above copyright notice,
+ *   this list of conditions and the following disclaimer in the documentation
+ *   and/or other materials provided with the distribution.
+ * - The names of contributors may not be used to endorse or promote products
+ *   derived from this software without specific prior written permission.
+ *
+ * THIS SOFTWARE IS PROVIDED BY THE COPYRIGHT HOLDERS AND CONTRIBUTORS "AS IS"
+ * AND ANY EXPRESS OR IMPLIED WARRANTIES, INCLUDING, BUT NOT LIMITED TO, THE
+ * IMPLIED WARRANTIES OF MERCHANTABILITY AND FITNESS FOR A PARTICULAR PURPOSE
+ * ARE DISCLAIMED. IN NO EVENT SHALL THE COPYRIGHT OWNER OR CONTRIBUTORS BE
+ * LIABLE FOR ANY DIRECT, INDIRECT, INCIDENTAL, SPECIAL, EXEMPLARY, OR 
+ * CONSEQUENTIAL DAMAGES (INCLUDING, BUT NOT LIMITED TO, PROCUREMENT OF
+ * SUBSTITUTE GOODS OR SERVICES; LOSS OF USE, DATA, OR PROFITS; OR BUSINESS
+ * INTERRUPTION) HOWEVER CAUSED AND ON ANY THEORY OF LIABILITY, WHETHER IN
+ * CONTRACT, STRICT LIABILITY, OR TORT (INCLUDING NEGLIGENCE OR OTHERWISE)
+ * ARISING IN ANY WAY OUT OF THE USE OF THIS SOFTWARE, EVEN IF ADVISED OF THE
+ * POSSIBILITY OF SUCH DAMAGE.
+ *)
+
+type 'a axiom_ST = unit -> 'a
+
+let axiom_STBind b k () = let v = b () in k v ()
+
+let axiom_STReturn v () = v
+
+let axiom_STContra () = failwith "ST Contradiction"
+
+let axiom_STWeaken x = x
+
+let axiom_STStrengthen x = x
+ 
+let axiom_STNew v () = ref (Obj.repr v)
+
+let axiom_STFree _ () = ()
+
+let axiom_STRead p () = Obj.obj !p
+
+let axiom_STWrite p v () = p := Obj.repr v
+
+(** ((a -> (unit -> b)) -> a -> (unit -> b)) -> a -> (unit -> b) **)
+let axiom_STFix f = 
+  let rec fix a () = f fix a ()
+  in fix
+
+let exec io = io ()
