compiler/dsl/coq/ReflexIO.v
@@ -8,84 +8,13 @@ Open Scope char_scope.
 Open Scope hprop_scope.
 Open Scope stsepi_scope.
 
+Require Import ReflexBase.
+
 Ltac sep' := sep fail idtac.
-Ltac inv H := inversion H; subst; clear H.
-
-(* follow ascii design, little endian *)
-Inductive Num : Set :=
-| num : ascii -> ascii -> Num.
-
-Definition nat_of_Num (n : Num) : nat :=
-  match n with
-  | num l h => nat_of_ascii l + nat_of_ascii h * 256
-  end.
-
-Definition Num_of_nat (n : nat) : Num :=
-  let l := n mod 256 in
-  let h := n / 256 in
-  num (ascii_of_nat l) (ascii_of_nat h).
-
-Lemma nat_of_ascii_bound :
-  forall x, nat_of_ascii x < 256.
-Proof.
-  destruct x.
-  repeat (
-    match goal with [ b : bool |- _ ] => destruct b end
-  ); compute; omega.
-Qed.
-
-Lemma Num_nat_embedding :
-  forall (n : Num), Num_of_nat (nat_of_Num n) = n.
-Proof with try discriminate.
-  destruct n as [[l h]]; simpl.
-  unfold Num_of_nat, nat_of_Num.
-  repeat f_equal.
-  rewrite mod_add... rewrite mod_small. now rewrite ascii_nat_embedding.
-  apply nat_of_ascii_bound.
-  rewrite div_add... rewrite div_small. simpl. now rewrite ascii_nat_embedding.
-  apply nat_of_ascii_bound.
-Qed.
-
-Definition Num_eq (n1 n2 : Num) : {n1 = n2} + {n1 <> n2}.
-  decide equality; apply ascii_dec.
-Qed.
-
-(* prevent sep tactic from unfolding *)
-Global Opaque nat_of_Num Num_of_nat Num_eq.
-
-Definition Str : Set :=
-  list ascii.
-
-Fixpoint str_of_string (s : string) : Str :=
-  match s with
-  | EmptyString => nil
-  | String c rest => c :: str_of_string rest
-  end.
-
-Definition FD : Set :=
-  Num.
-
-Definition FD_eq (f1 f2 : FD) : {f1 = f2} + {f1 <> f2} :=
-  Num_eq f1 f2.
-
-Lemma FD_eq_true :
-  forall (f : FD) (A : Type) (vT vF : A),
-  (if FD_eq f f then vT else vF) = vT.
-Proof.
-  intros; case (FD_eq f f); auto. congruence.
-Qed.
-
-Lemma FD_eq_false :
-  forall (f1 f2 : FD) (A : Type) (vT vF : A),
-  f1 <> f2 ->
-  (if FD_eq f1 f2 then vT else vF) = vF.
-Proof.
-  intros; case (FD_eq f1 f2); auto. congruence.
-Qed.
 
 Inductive Action : Set :=
-| Exec   : Str -> FD -> Action
-| Call   : Str -> Str -> FD -> Action
+| Exec   : Str -> list Str -> FD -> Action
+| Call   : Str -> list Str -> FD -> Action
 | Select : list FD -> FD -> Action
 | Recv   : FD -> Str -> Action
 | Send   : FD -> Str -> Action
@@ -109,14 +38,14 @@ Definition CallPerms : list Perm :=
 Axiom open : FD -> list Perm -> hprop.
 
 Axiom exec :
-  forall (prog : Str) (tr : [Trace]),
+  forall (prog : Str) (args : list Str) (tr : [Trace]),
     STsep (tr ~~ traced tr)
-          (fun f : FD => tr ~~ open f ExecPerms * traced (Exec prog f :: tr)).
+          (fun f : FD => tr ~~ open f ExecPerms * traced (Exec prog args f :: tr)).
 
 Axiom call :
-  forall (prog arg : Str) (tr : [Trace]),
+  forall (prog : Str) (args : list Str) (tr : [Trace]),
   STsep (tr ~~ traced tr)
-        (fun f : FD => tr ~~ open f CallPerms * traced (Call prog arg f :: tr)).
+        (fun f : FD => tr ~~ open f CallPerms * traced (Call prog args f :: tr)).
 
 (* TODO add non-empty precondition *)
 (* TODO add open w/ recv perms precondition *)
