compiler/dsl/coq/Extract.v
@@ -1,0 +1,15 @@
+Require Import Ynot.Extract.
+Require Import Reflex.
+
+Extraction Blacklist List String.
+
+Extract Constant ReflexIO.exec     => "ReflexImpl.exec".
+Extract Constant ReflexIO.call     => "ReflexImpl.call".
+Extract Constant ReflexIO.select   => "ReflexImpl.select".
+Extract Constant ReflexIO.recv     => "ReflexImpl.recv".
+Extract Constant ReflexIO.send     => "ReflexImpl.send".
+Extract Constant ReflexIO.recv_fd  => "ReflexImpl.recv_fd".
+Extract Constant ReflexIO.send_fd  => "ReflexImpl.send_fd".
+
+Cd "../ml".
+Recursive Extraction Library Reflex.
