compiler/dsl/coq/ReflexBase.v
@@ -1,0 +1,81 @@
+Require Import List.
+Require Import Ascii.
+Require Import String.
+Require Import NPeano.
+Require Import Ynot.
+
+Open Scope char_scope.
+Open Scope hprop_scope.
+Open Scope stsepi_scope.
+
+(* follow ascii design, little endian *)
+Inductive Num : Set :=
+| num : ascii -> ascii -> Num.
+
+Definition nat_of_Num (n : Num) : nat :=
+  match n with
+  | num l h => nat_of_ascii l + nat_of_ascii h * 256
+  end.
+
+Definition Num_of_nat (n : nat) : Num :=
+  let l := n mod 256 in
+  let h := n / 256 in
+  num (ascii_of_nat l) (ascii_of_nat h).
+
+Lemma nat_of_ascii_bound :
+  forall x, nat_of_ascii x < 256.
+Proof.
+  destruct x.
+  repeat (
+    match goal with [ b : bool |- _ ] => destruct b end
+  ); compute; omega.
+Qed.
+
+Lemma Num_nat_embedding :
+  forall (n : Num), Num_of_nat (nat_of_Num n) = n.
+Proof with try discriminate.
+  destruct n as [[l h]]; simpl.
+  unfold Num_of_nat, nat_of_Num.
+  repeat f_equal.
+  rewrite mod_add... rewrite mod_small. now rewrite ascii_nat_embedding.
+  apply nat_of_ascii_bound.
+  rewrite div_add... rewrite div_small. simpl. now rewrite ascii_nat_embedding.
+  apply nat_of_ascii_bound.
+Qed.
+
+Definition Num_eq (n1 n2 : Num) : {n1 = n2} + {n1 <> n2}.
+  decide equality; apply ascii_dec.
+Qed.
+
+Definition Str : Set :=
+  list ascii.
+
+Fixpoint str_of_string (s : string) : Str :=
+  match s with
+  | EmptyString => nil
+  | String c rest => c :: str_of_string rest
+  end.
+
+Definition FD : Set :=
+  Num.
+
+Definition FD_eq (f1 f2 : FD) : {f1 = f2} + {f1 <> f2} :=
+  Num_eq f1 f2.
+
+Lemma FD_eq_true :
+  forall (f : FD) (A : Type) (vT vF : A),
+  (if FD_eq f f then vT else vF) = vT.
+Proof.
+  intros; case (FD_eq f f); auto. congruence.
+Qed.
+
+Lemma FD_eq_false :
+  forall (f1 f2 : FD) (A : Type) (vT vF : A),
+  f1 <> f2 ->
+  (if FD_eq f1 f2 then vT else vF) = vF.
+Proof.
+  intros; case (FD_eq f1 f2); auto. congruence.
+Qed.
+
+(* prevent sep tactic from unfolding *)
+Global Opaque nat_of_Num Num_of_nat.
